testdata/cue/comprehensions/list_comprehension_for_kv.cue
@@ -1,0 +1,1 @@
+out: [for k, v in {a: 1, b: 2} {v}]
