testdata/cue/comprehensions/list_comprehension_guard_for.cue
@@ -1,0 +1,2 @@
+l: [1, 2, 3, 4]
+out: [for x in l if x > 2 {x}]
