testdata/cue/comprehensions/list_comprehension_mixed.cue
@@ -1,0 +1,2 @@
+xs: [5, 6]
+out: [1, for x in xs {x}, 2]
