testdata/cue/comprehensions/list_comprehension_nested.cue
@@ -1,0 +1,3 @@
+xs: [1, 2]
+ys: [10, 20]
+out: [for x in xs for y in ys {x + y}]
